Completed the proof of the current refinement.

Isabelle2/AbstractMultiPaxosR1.thy
@@ -3,14 +3,20 @@ imports  "../../IO-Automata/IOA" BallotArrays3 DistributedSafeAt
 begin
 
 text {* 
-1) added a suggestions that acceptors then vote for, and used the distributed implementation of the safe-at computation.
+1) Acceptors vote for a suggestion, and leaders use the distributed implementation of the safe-at computation.
+2) Explicit 1b messages.
 *}
+
+type_synonym bal = nat
+type_synonym inst = nat
+text {* TODO: how to use and real type and the transfer package? *}
 
 record ('v,'a) amp_state =
   propCmd :: "'v set"
-  ballot :: "'a \<Rightarrow> nat"
-  vote :: "nat \<Rightarrow> 'a \<Rightarrow> nat \<rightharpoonup> 'v"
-  suggestion :: "nat \<Rightarrow> nat \<rightharpoonup> 'v"
+  ballot :: "'a \<Rightarrow> bal"
+  vote :: "inst \<Rightarrow> 'a \<Rightarrow> bal \<rightharpoonup> 'v"
+  suggestion :: "inst \<Rightarrow> bal \<rightharpoonup> 'v"
+  onebs :: "'a \<Rightarrow> bal \<rightharpoonup> (inst \<rightharpoonup> ('v\<times>bal))"
 
 locale amp_ioa = IOA +
   fixes quorums::"'a set set"
@@ -31,7 +37,7 @@ definition amp_asig where
 definition amp_start where
   -- {* The initial state *}
   "amp_start \<equiv> {\<lparr>propCmd = {}, ballot = (\<lambda> a . 0), vote = (\<lambda> i a . Map.empty), 
-    suggestion = \<lambda> i . Map.empty \<rparr>}"
+    suggestion = \<lambda> i . Map.empty, onebs = \<lambda> a . Map.empty \<rparr>}"
 
 subsection {* The transitions *}
 
@@ -39,22 +45,21 @@ definition propose where
   "propose c r r' \<equiv> (r' = r\<lparr>propCmd := (propCmd r) \<union> {c}\<rparr>)"
 
 definition join_ballot where
-  "join_ballot a b s s' \<equiv>
-    b > (ballot s a) \<and> s' = s\<lparr>ballot := (ballot s)(a := b)\<rparr>"
-
-abbreviation proved_safe_at where 
-  -- {* v is proved safe in instance i at ballot b by quorum q *}
-  "proved_safe_at s i q b v \<equiv> distributed_safe_at.proved_safe_at (ballot s) (vote s i) quorums q b v"
-
-abbreviation conservative_at where
-  "conservative_at s i \<equiv> ballot_array.conservative_array (vote s i)"
+  "join_ballot a b s s' \<equiv> 
+    let onebs' = \<lambda> i . distributed_safe_at.acc_max (vote s i) a b
+    in
+      b > (ballot s a) \<and> s' = s\<lparr>ballot := (ballot s)(a := b),
+        onebs := (onebs s)(a := (onebs s a)(b \<mapsto> onebs'))\<rparr>"
 
 definition suggest where
   "suggest i b v q s s' \<equiv>
-          v \<in> propCmd s 
+          v \<in> propCmd s
         \<and> suggestion s i b = None
-        \<and> proved_safe_at s i q b v
-        \<and> s' = s\<lparr>suggestion := (suggestion s)(i := (suggestion s i)(b \<mapsto> v))\<rparr>"
+        \<and> q \<in> quorums
+        \<and> (\<forall> a \<in> q . onebs s a b \<noteq> None)
+        \<and> (let m = distributed_safe_at.max_pair q (\<lambda> a . the (onebs s a b) i) in 
+            (case m of None \<Rightarrow> True | Some (v',b') \<Rightarrow> v = v')
+            \<and> s' = s\<lparr>suggestion := (suggestion s)(i := (suggestion s i)(b \<mapsto> v))\<rparr>)"
 
 definition do_vote where
   "do_vote a i v s s' \<equiv> let b = ballot s a in
@@ -71,12 +76,12 @@ definition learn where
 fun amp_trans_rel where
   "amp_trans_rel r (Propose c) r' = propose c r r'"
 | "amp_trans_rel r Internal r' = (
-    (\<exists> a b . join_ballot a b r r') 
+    (\<exists> a b . join_ballot a b r r')
     \<or> (\<exists> a i v . do_vote a i v r r')
     \<or> (\<exists> i b v q . suggest i b v q r r'))"
 | "amp_trans_rel r (Learn i v l) r' = learn i v r r'"
 
-lemma trans_cases[consumes 1]: 
+lemma trans_cases[consumes 1]:
   assumes "amp_trans_rel r a r'"
   obtains 
   (propose) c where "propose c r r'"
