Isabelle2/AbstractMultiPaxosR1Correctness.thy
@@ -48,14 +48,12 @@ apply (simp_all add:inv1_def)
 by (metis option.simps(3))
 declare inv1[invs]
 
-abbreviation safe_at where "safe_at s i \<equiv> ballot_array.safe_at quorums (ballot s) (vote s i)"
-
-declare 
+declare
   ballot_array.conservative_array_def[inv_proofs_defs]
   ballot_array.conservative_def[inv_proofs_defs]
 
 abbreviation conservative_array where
-"conservative_array s \<equiv>  \<forall> i . conservative_at s i"
+  "conservative_array s \<equiv>  \<forall> i . ballot_array.conservative_array (vote s i)"
 
 lemma conservative:
   "invariant the_ioa conservative_array"
@@ -79,11 +77,53 @@ lemma trans_imp_prefix_order:
   apply (auto simp add:is_prefix_def inv_proofs_defs split add:option.split_asm)
 done
 
+abbreviation safe_at where "safe_at s i \<equiv> ballot_array.safe_at quorums (ballot s) (vote s i)"
+
 lemma safe_mono:
   -- {* @{term safe_at} is monotonic. *}
   assumes "s \<midarrow>a\<midarrow>the_ioa\<longrightarrow> t" and "safe_at s i v b"
   shows "safe_at t i v b" using assms ballot_array_prefix.safe_at_mono
-by (metis ballot_array_prefix_axioms.intro ballot_array_prefix_def quorums_axioms trans_imp_prefix_order)
+by (metis ballot_array_prefix_axioms_def ballot_array_prefix_def quorums_axioms trans_imp_prefix_order) 
+
+definition inv3 where 
+  inv3_def[inv_proofs_defs]:"inv3 s \<equiv> \<forall> a b . case onebs s a b of None \<Rightarrow> True
+    | Some maxs \<Rightarrow> 
+      (\<forall> i . maxs i = distributed_safe_at.acc_max (vote s i) a b)
+      \<and> (ballot s a \<ge> b)"
+
+lemma inv3:
+  "invariant the_ioa inv3"
+apply (rule invariantI)
+apply (force simp add:inv_proofs_defs)
+apply instantiate_invs_2
+apply (unfold_to_trans_rel)
+apply ((induct_tac rule:trans_cases, simp); rm_trans_rel_assm)
+          apply (auto simp add:inv_proofs_defs  split add:option.splits)[2]
+      defer defer apply (auto simp add:inv_proofs_defs  split add:option.splits)[2]
+      apply (metis dual_order.trans nat_less_le)
+  subgoal premises prems for s t act a i v
+  proof -
+    { fix a2 b maxs
+      assume a1:"onebs s a2 b = Some maxs"
+      from a1 prems(1) have 1:"\<And> j . maxs j = distributed_safe_at.acc_max (vote s j) a2 b" 
+        by (simp add:inv3_def split add:option.splits split_if split_if_asm)
+      from a1 prems(1,6) have 2:"ballot t a2 \<ge> b" by (simp add:inv3_def split add:option.splits)
+      { fix j assume "j \<noteq> i \<or> a \<noteq> a2"
+        hence "maxs j = distributed_safe_at.acc_max (vote t j) a2 b" using 1 prems(6) by (auto simp add:distributed_safe_at.acc_max_def) }
+      note 3 = this
+      { fix j assume "j = i \<and> a = a2"
+        hence "maxs j = distributed_safe_at.acc_max (vote t j) a2 b" using 1 prems(6) a1 2 apply (simp add:distributed_safe_at.acc_max_def)
+          by (smt Collect_cong amp_state.select_convs(2) amp_state.surjective amp_state.update_convs(3) dual_order.strict_trans1 neq_iff split_cong) }
+      note this 2 3 }
+    thus ?thesis apply (simp add:inv3_def split add:option.splits)
+      by (metis (no_types, lifting) amp_ioa.do_vote_def amp_state.select_convs(5) amp_state.surjective amp_state.update_convs(3) prems(6))
+  qed
+done
+declare inv3[invs]
+      
+(* nitpick[no_assms, show_consts, verbose, card 'a = 3, card 'v = 2, card nat = 2, card "'v option" = 3, card "nat option" = 3,
+    card "('v \<times> nat) option" = 5, card "'v \<times> nat" = 4, card unit = 1, card "('v, 'a) amp_state" = 32, card 'l = 1, expect=none]  *)
+          
 
 definition inv2 where
   -- {* a suggestion is safe. *}
@@ -99,19 +139,41 @@ apply (rule invariantI)
   apply instantiate_invs_2
   subgoal premises prems for s t a
   proof -
-    from prems and safe_mono have 1:"\<And> i v b . safe_at s i v b \<Longrightarrow> safe_at t i v b"
-      by (simp add:inv2_def)
+    from prems and safe_mono have 1:"\<And> i v b . safe_at s i v b \<Longrightarrow> safe_at t i v b" by (simp add:inv2_def)
     with prems show ?thesis
     apply (unfold_to_trans_rel)
     apply ((induct_tac rule:trans_cases, simp); rm_trans_rel_assm)
               apply (auto simp add:inv_proofs_defs split add:option.splits)[3]
         apply (fastforce simp add:inv_proofs_defs split add:option.splits)
-      apply auto
+        apply clarify
       subgoal premises prems for i b v q
       proof -
-        from prems(5,8,2) have "safe_at s i v b"
-          by (smt ballot_array.safe_def distributed_safe_at.intro distributed_safe_at.proved_safe_at_imp_safe_at option.case_eq_if option.distinct(1) option.sel quorums_axioms) 
-        thus ?thesis using prems(4,9) 1 by (simp add:inv2_def split add:option.splits)
+        from \<open>safe s\<close> \<open>suggest i b v q s t\<close> have "safe t" by (metis amp_state.select_convs(2) amp_state.select_convs(3) amp_state.surjective amp_state.update_convs(4) suggest_def) 
+        moreover have "inv2 t"
+        proof (auto simp add: inv2_def split add:option.split)
+          fix j b2 w
+          assume "suggestion t j b2 = Some w"
+          show "safe_at t j w b2"
+          proof (cases "i \<noteq> j \<or> b2 \<noteq> b")
+            case True
+            thus "safe_at t j w b2" using \<open>inv2 s\<close> \<open>suggest i b v q s t\<close>  apply (simp add:inv2_def split add:option.splits)
+              apply (smt \<open>suggestion t j b2 = Some w\<close> amp_state.ext_inject amp_state.surjective amp_state.update_convs(4) fun_upd_def)
+              by (smt \<open>suggestion t j b2 = Some w\<close> amp_state.ext_inject amp_state.surjective amp_state.update_convs(4) fun_upd_def)
+          next
+            case False
+            hence "v = w" using \<open>suggest i b v q s t\<close>  \<open>suggestion t j b2 = Some w\<close> by simp
+            have 2:"\<And> a . a \<in> q \<Longrightarrow> b \<le> ballot s a" using  \<open>suggest i b v q s t\<close> \<open>inv3 s\<close> by (auto simp add:inv3_def split add:option.splits)
+            have 1:"\<And> a . a \<in> q \<Longrightarrow> case onebs s a b of Some f \<Rightarrow> f i = distributed_safe_at.acc_max (vote s i) a b | None \<Rightarrow> False" 
+              using \<open> suggest i b v q s t\<close> \<open>inv3 s\<close> by (simp add:inv3_def split add:option.splits)
+            hence 3:"distributed_safe_at.max_pair q (\<lambda> a . the (onebs s a b) i) = distributed_safe_at.max_pair q (\<lambda> a . distributed_safe_at.acc_max (vote s i) a b)"
+              apply (simp add:distributed_safe_at.max_pair_def split add:option.splits) by (smt SUP_def image_cong option.case_eq_if)
+            have "distributed_safe_at.proved_safe_at quorums (ballot s) (vote s i) q b v" using 1 2 3 \<open>suggest i b v q s t\<close> \<open>v = w\<close> 
+              by (auto simp add:distributed_safe_at.proved_safe_at_def split add:option.splits)
+            interpret p:dsa_properties "ballot s" "vote s i" quorums by unfold_locales
+            show ?thesis by (metis False \<open>p.proved_safe_at q b v\<close> \<open>v = w\<close> option.simps(5) p.proved_safe_at_imp_safe_at p.safe_def prems(10) prems(2) prems(7)) 
+          qed
+        qed
+        ultimately show ?thesis by auto
       qed
     done
   qed
